theories/RenameApartToPart.v
@@ -1,111 +1,83 @@
 Require Import Util CSet IL Annotation StableFresh InfinitePartition VarP.
-Require Import RenameApart RenamedApartAnn RenameApart_VarP Fresh Range Setoid.
+Require Import RenameApart RenamedApartAnn RenameApart_VarP FreshGen Range Setoid.
 
-
-Definition FG_fast : FreshGen nat :=
-  @Build_FreshGen nat
-                  (fun n _ => (n, S n))
-                  (fun n Z => (range n ❬Z❭, n + ❬Z❭))
-                  nats_up_to
-                  (fun n s => max n (S (fold Init.Nat.max s 0))).
-
-Lemma nats_up_to_in x i
-  : x < i <-> x ∈ nats_up_to i.
-Proof.
-  induction i; simpl.
-  - split. omega. cset_tac.
-  - decide (x = i); subst.
-    + split. cset_tac. omega.
-    + split; intros.
-      -- cset_tac'. eapply H0. omega.
-      -- cset_tac'.
-Qed.
-
-Lemma range_nodup i d
-  : NoDupA eq (range i d).
-Proof.
-  general induction d; simpl; eauto using NoDupA.
-  econstructor; eauto.
-  intro. eapply InA_eq_of_list in H.
-  eapply in_range_x in H. omega.
-Qed.
-
-
-Lemma FGS_fast : FreshGenSpec FG_fast.
-  econstructor; simpl.
-  - intros. rewrite <- nats_up_to_in. omega.
-  - reflexivity.
-  - intros; hnf; intros.
-    eapply nats_up_to_in in H.
-    eapply in_range_x in H0 as [? ?]. omega.
-  - intros. cset_tac'.
-    + rewrite <- nats_up_to_in in *.
-      eapply x_notin_range in n. omega.
-    + rewrite <- nats_up_to_in in *.
-      eapply in_range_x in H0. omega.
-    + rewrite <- nats_up_to_in in *. omega.
-  - intros. eapply range_nodup.
-  - eauto with len.
-  - simpl. cset_tac'.
-    eapply nats_up_to_in.
-    + rewrite <- Max.le_max_r.
-      eapply fresh_spec' in H0. omega.
-    + eapply nats_up_to_in in H0.
-      eapply nats_up_to_in.
-      rewrite <- Max.le_max_l. eauto.
-Qed.
+Set Implicit Arguments.
 
 Definition rename_apart_to_part {Fi} (FG:FreshGen Fi) (FGS:FreshGenSpec FG) fi (s:stmt) :=
-  let (xl, fi) := (fresh_list FG fi (to_list (freeVars s))) in
-  let s' := (renameApart' FG fi
-                       (id [to_list (freeVars s) <-- xl])
+  let xlfi := (fresh_list FG fi (to_list (freeVars s))) in
+  let s' := (renameApart' FG (snd xlfi)
+                       (id [to_list (freeVars s) <-- fst xlfi])
                        s) in
-  (snd s', renamedApartAnn (snd s') (of_list xl)).
+  (snd s', renamedApartAnn (snd s') (of_list (fst xlfi))).
 
 Opaque to_list.
 
-Lemma rename_apart_to_part_renamedApart s
-  : RenamedApart.renamedApart (fst (rename_apart_to_part s))
-                              (snd (rename_apart_to_part s)).
+Lemma rename_apart_to_part_renamedApart {Fi} (FG:FreshGen Fi) (FGS:FreshGenSpec FG) fi s
+  : RenamedApart.renamedApart (fst (rename_apart_to_part FGS fi s))
+                              (snd (rename_apart_to_part FGS fi s)).
 Proof.
   unfold rename_apart_to_part. simpl.
-  eapply renameApart'_renamedApart.
+  eapply renameApart'_renamedApart; eauto.
   - rewrite update_with_list_lookup_set_incl; eauto with len.
+    rewrite fresh_list_len; eauto.
     rewrite of_list_3; eauto.
-  - reflexivity.
+  - rewrite <- fresh_list_domain_spec; eauto with cset.
 Qed.
 
 
-Lemma rename_apart_to_part_occurVars s
-  : fst (getAnn (snd (rename_apart_to_part s)))
-        ∪ snd (getAnn (snd (rename_apart_to_part s)))
-        [=] occurVars (fst (rename_apart_to_part s)).
+Lemma rename_apart_to_part_occurVars {Fi} (FG:FreshGen Fi) (FGS:FreshGenSpec FG) fi s
+  : fst (getAnn (snd (rename_apart_to_part FGS fi s)))
+        ∪ snd (getAnn (snd (rename_apart_to_part FGS fi s)))
+        [=] occurVars (fst (rename_apart_to_part FGS fi s)).
 Proof.
   unfold rename_apart_to_part; simpl.
   rewrite occurVars_freeVars_definedVars.
   rewrite snd_renamedApartAnn.
   eapply eq_union_lr; eauto.
   rewrite fst_renamedApartAnn.
-  rewrite freeVars_renamedApart'.
+  rewrite freeVars_renamedApart'; eauto.
   - rewrite update_with_list_lookup_list_eq; eauto with len.
+    + rewrite fresh_list_len; eauto.
     + eapply nodup_to_list_eq.
     + rewrite of_list_3; eauto.
   - rewrite update_with_list_lookup_list_eq; eauto with len.
+    + rewrite <- fresh_list_domain_spec; eauto.
+    + rewrite fresh_list_len; eauto.
     + eapply nodup_to_list_eq.
     + rewrite of_list_3; eauto.
 Qed.
 
-Lemma rename_to_subset_even (s:stmt)
+Lemma FG_even_fast_inf_subset fi x
+  :  even_inf_subset (fst (FG_even_fast fi x)).
+Proof.
+  hnf. simpl. destruct fi; simpl. cases; eauto.
+Qed.
+
+Lemma even_fast_list_even fi
+  :  forall Z x, x \In of_list (fst (fresh_list FG_even_fast fi Z)) ->
+            even_inf_subset x.
+Proof.
+  intros.
+  unfold fresh_list in H. simpl in *.
+  eapply of_list_map in H; eauto. cset_tac'.
+  eapply of_list_map in H; eauto. cset_tac'.
+  eapply in_range_x in H as [? ?]. destruct fi; simpl in *.
+  eapply even_add; eauto. eapply even_mult2.
+Qed.
+
+Lemma rename_to_subset_even fi s
   : For_all (inf_subset_P even_inf_subset)
-            (occurVars (fst (rename_apart_to_part s))).
+            (occurVars (fst (rename_apart_to_part FGS_even_fast fi s))).
 Proof.
   eapply var_P_occurVars.
-  eapply renameApart_var_P.
-  - intros. eapply least_fresh_P_full_spec.
+  eapply renameApart_var_P; eauto using FGS_even_fast.
+  - intros. eapply FG_even_fast_inf_subset.
   - intros.
-    edestruct update_with_list_lookup_in_list; dcr.
-    Focus 3. rewrite H3. hnf in H5. subst.
-    exploit fresh_list_stable_get; eauto; dcr; subst.
-    eapply least_fresh_P_full_spec.
-    eauto with len. rewrite of_list_3; eauto.
+    eapply even_fast_list_even; eauto.
+  - intros. rewrite <- of_list_3 in H.
+    eapply (update_with_list_lookup_in_list id _ (fst (fresh_list FG_even_fast fi (to_list (freeVars s))))) in H; dcr.
+    + rewrite H2.
+      eapply even_fast_list_even.
+      eapply get_in_of_list; eauto.
+    + rewrite fresh_list_len; eauto using FGS_even_fast.
 Qed.
