theories/Alpha/RenameApart_Alpha.v
@@ -1,11 +1,11 @@
 Require Import CSet Util Map.
 Require Import Env IL Alpha Annotation RenamedApart SetOperations.
-Require Import LabelsDefined PairwiseDisjoint RenameApart.
+Require Import LabelsDefined PairwiseDisjoint RenameApart FreshGen.
 
 Set Implicit Arguments.
 
 Lemma rename_apart_alpha' {Fi} (FG:FreshGen Fi) (FGS:FreshGenSpec FG) fi ϱ ϱ' s
-  : lookup_set ϱ (freeVars s) ⊆ domain _ fi
+  : lookup_set ϱ (freeVars s) ⊆ domain FG fi
   -> inverse_on (freeVars s) ϱ ϱ'
   -> alpha ϱ' ϱ (snd (renameApart' FG fi ϱ s)) s.
 Proof.
@@ -85,6 +85,6 @@ Lemma rename_apart_alpha {Fi} (FG:FreshGen Fi) (FGS:FreshGenSpec FG) fi s
   : alpha id id (rename_apart FG (domain_add FG fi (freeVars s)) s) s.
 Proof.
   eapply rename_apart_alpha'; eauto.
-  + eapply lookup_set_on_id. rewrite domain_add_spec; eauto with cset.
+  + eapply lookup_set_on_id. rewrite <- domain_add_spec; eauto with cset.
   + eapply inverse_on_id.
 Qed.
