theories/Infra/FreshGen.v
@@ -1,0 +1,169 @@
+Require Import CSet Le Arith.Compare_dec.
+Require Import Plus Util Map Get Take LengthEq SafeFirst.
+Require Export StableFresh Fresh Range InfinitePartition.
+
+Set Implicit Arguments.
+
+Inductive FreshGen (Fi : Type) :=
+  {
+    fresh :> Fi -> nat -> nat * Fi;
+    fresh_list : Fi -> list nat -> list nat * Fi;
+    domain : Fi -> set nat;
+    domain_add : Fi -> set nat -> Fi
+  }.
+
+Inductive FreshGenSpec Fi (FG:FreshGen Fi) : Prop :=
+  {
+    fresh_spec : forall i x, fst (fresh FG i x) ∉ domain FG i;
+    fresh_domain_spec : forall i x, {fst (fresh FG i x); (domain FG i)}
+                                 ⊆ domain FG (snd (fresh FG i x));
+    fresh_list_disj : forall i Z, disj (domain FG i) (of_list (fst (fresh_list FG i Z)));
+    fresh_list_domain_spec : forall i Z, of_list (fst (fresh_list FG i Z)) ∪ domain FG i
+                                            ⊆ domain FG (snd (fresh_list FG i Z));
+    fresh_list_nodup : forall i Z, NoDupA eq (fst (fresh_list FG i Z));
+    fresh_list_len : forall i Z, ❬fst (fresh_list FG i Z)❭ = ❬Z❭;
+    domain_add_spec : forall i G, G ∪ domain FG i ⊆ domain FG (domain_add FG i G)
+  }.
+
+Create HintDb fresh discriminated.
+
+
+Definition FG_fast : FreshGen nat :=
+  @Build_FreshGen nat
+                  (fun n _ => (n, S n))
+                  (fun n Z => (range n ❬Z❭, n + ❬Z❭))
+                  nats_up_to
+                  (fun n s => max n (S (fold Init.Nat.max s 0))).
+
+
+Lemma FGS_fast : FreshGenSpec FG_fast.
+  econstructor; simpl.
+  - intros. rewrite <- nats_up_to_in. omega.
+  - reflexivity.
+  - intros; hnf; intros.
+    eapply nats_up_to_in in H.
+    eapply in_range_x in H0 as [? ?]. omega.
+  - intros. cset_tac'.
+    + rewrite <- nats_up_to_in in *.
+      eapply in_range_x in H0. omega.
+    + rewrite <- nats_up_to_in in *. omega.
+  - intros. eapply range_nodup.
+  - eauto with len.
+  - simpl. cset_tac'.
+    eapply nats_up_to_in.
+    + rewrite <- Max.le_max_r.
+      eapply fresh_spec' in H0. omega.
+    + eapply nats_up_to_in in H0.
+      eapply nats_up_to_in.
+      rewrite <- Max.le_max_l. eauto.
+Qed.
+
+Definition next_even (n:nat) := if [even n] then n else S n.
+
+Lemma next_even_even n
+  : even (next_even n).
+Proof.
+  unfold next_even; cases; eauto.
+  edestruct (even_or_successor n); eauto.
+Qed.
+
+Lemma even_add x y
+  : even x
+    -> even y
+    -> even (x + y).
+Proof.
+  revert y. pattern x.
+  eapply size_induction with (f:=id); intros.
+  destruct x0; simpl; eauto.
+  destruct x0; simpl; eauto.
+  eapply H; eauto. unfold id. omega.
+Qed.
+
+Lemma even_max x y
+  : even x
+    -> even y
+    -> even (max x y).
+Proof.
+  intros.
+  decide (x < y).
+  - rewrite max_r; try omega; eauto.
+  - rewrite max_l; try omega; eauto.
+Qed.
+
+Lemma even_mult2 x
+  : even (2 * x).
+Proof.
+  pattern x.
+  eapply size_induction with (f:=id); intros.
+  destruct x0; simpl; eauto.
+  destruct x0; simpl; eauto. rewrite plus_comm. simpl.
+  rewrite <- plus_assoc. simpl.
+  exploit (H x0).
+  - unfold id. omega.
+  - simpl in H0. setoid_rewrite plus_comm in H0 at 2. simpl in *. eauto.
+Qed.
+
+Definition FG_even_fast : FreshGen {n | even n}.
+  refine
+    (@Build_FreshGen {n | even n}
+                  (fun n _ => (proj1_sig n, exist _ (S (S (proj1_sig n))) _))
+                  (fun n Z => let z := 2 * ❬Z❭ in
+                     (plus (proj1_sig n) ⊝ mult 2 ⊝ range 0 ❬Z❭, exist _ (proj1_sig n + z) _))
+                  (fun n => nats_up_to (proj1_sig n))
+                  (fun n s =>
+                     exist _ (max (proj1_sig n) (next_even (S (fold Init.Nat.max s 0)))) _)).
+  - simpl. destruct n. eauto.
+  - destruct n. subst z.
+    eapply even_add; eauto.
+    eapply even_mult2.
+  - destruct n. eapply even_max; eauto using next_even_even.
+Defined.
+
+Lemma NoDup_inj A `{OrderedType A} B `{OrderedType B} (L:list A) (f:A -> B)
+      `{Proper _ (_eq ==> _eq) f}
+  : NoDupA _eq L
+    -> injective_on (of_list L) f
+    -> NoDupA _eq (f ⊝ L).
+Proof.
+  intros ND INJ.
+  general induction ND; simpl in *; eauto using NoDupA.
+  econstructor; eauto using injective_on_incl with cset.
+  intro. eapply InA_in in H3.
+  eapply H0. eapply of_list_map in H3; eauto. cset_tac'.
+  eapply INJ in H4; eauto with cset.
+Qed.
+
+Lemma FGS_even_fast : FreshGenSpec FG_even_fast.
+  econstructor; simpl.
+  - intros. rewrite <- nats_up_to_in. omega.
+  - intros [] _; simpl. cset_tac.
+  - intros; hnf; intros.
+    eapply nats_up_to_in in H.
+    eapply of_list_map in H0; eauto.
+    cset_tac'.
+    eapply of_list_map in H0; eauto.
+    cset_tac'.
+    eapply in_range_x in H0 as [? ?]. omega.
+  - intros. cset_tac'.
+    + eapply of_list_map in H0; eauto. cset_tac'.
+      eapply of_list_map in H; eauto. cset_tac'.
+      eapply in_range_x in H as [? ?].
+      rewrite <- nats_up_to_in in *. simpl in *. omega.
+    + rewrite <- nats_up_to_in in *. omega.
+  - intros. rewrite map_map.
+    exploit (@NoDup_inj nat _ nat _ (range 0 ❬Z❭)); swap 1 4.
+    eapply H.
+    eapply range_nodup.
+    hnf; intros. invc H1. hnf. omega.
+    eauto.
+  - eauto with len.
+  - simpl. cset_tac'.
+    eapply nats_up_to_in.
+    + rewrite <- Max.le_max_r. unfold next_even.
+      simpl in *.
+      eapply fresh_spec' in H0.
+      cases; eauto. omega. omega.
+    + eapply nats_up_to_in in H0.
+      eapply nats_up_to_in.
+      rewrite <- Max.le_max_l. eauto.
+Qed.
